Add comments and nicely format the code

Chen/Unproductive.thy
@@ -9,13 +9,12 @@ hide_const (open) Topological_Spaces.closed
 
 text \<open>Unproductive Symbol Elimination\<close>
 
-(* I think the inductive set definition is better, because we may want to use
-producthive.induct at some point *)
+(* I think we might prefer the inductive set definition, because we may want to
+use productive.induct at some point, although I'm not 100% sure *)
 inductive_set productive :: "('n,'t)Prods \<Rightarrow> 'n set" for P where
 "\<lbrakk> (A,\<alpha>) \<in> P; \<And>B. B \<in> nts_of_syms \<alpha> \<Longrightarrow> B \<in> productive P \<rbrakk> \<Longrightarrow> A \<in> productive P"
-print_theorems
 
-definition "rm_unproductive P = {(A,\<alpha>) \<in> P. A \<in> productive P}"
+definition "rm_unproductive P = {(A,\<alpha>) \<in> P. ({A} \<union> nts_of_syms \<alpha>) \<subseteq> productive P}"
 
 
 theorem "Lang (rm_unproductive P) A = Lang P A"
@@ -34,11 +33,21 @@ theorem "Lang (rm_unproductive P) A = Lang P A"
             assume "w \<in> Lang P A"
             then have "P \<turnstile> [Nt A] \<Rightarrow>* map Tm w"
               unfolding Lang_def by simp
+
+            (* should follow from A \<in> productive P, but I couldn't figure it out *)
             then have "rm_unproductive P \<turnstile> [Nt A] \<Rightarrow>* map Tm w"
-            sorry
+              using \<open>A \<in> productive P\<close>
+              proof (induction rule: rtrancl_derive_induct)
+                case base
+                then show ?case by simp
+              next
+                case (step u A' v w')
+                then show ?case 
+                sorry
+              qed
 
             then show "w \<in> Lang (rm_unproductive P) A"
-            sorry
+            by (simp add: Lang_def)
           qed
         then show ?thesis
           by auto
@@ -61,21 +70,18 @@ theorem "Lang (rm_unproductive P) A = Lang P A"
               case (step y z)
               then obtain \<alpha> \<beta> \<gamma> A' where "y = \<alpha> @ [Nt A'] @ \<gamma>" and "z = \<alpha> @ \<beta> @ \<gamma>"
                 by (meson derive.cases)
-              (* easily proved with an additional lemma*)
+              (* should be easily proved with an additional lemma*)
               then have "A' \<notin> productive P"
-              using \<open>A \<notin> productive P\<close> step.hyps unfolding productive_def 
-              sorry
-              show ?case
-                proof (rule ccontr)
-                  assume "\<not>({A. Nt A \<in> set z} \<noteq> {})"
-                  (* then have "y \<in> productive P" *)
-                  then show False
+              using \<open>A \<notin> productive P\<close> step.hyps sorry
+              (* I feel like this should follow from the previous statement,
+              but I wasn't able to prove it *)
+              then show ?case
                 sorry
-              qed
             qed
-          
+
           ultimately show False
             by simp
+
         qed
         then show ?thesis
           by auto
