Chen/Unreachable.thy
@@ -9,23 +9,40 @@ hide_const (open) Topological_Spaces.closed
 
 text \<open>Unreachable Symbol Elimination\<close>
 
-definition "reachable P A = (\<exists> B \<alpha> \<beta>. (B,\<alpha> @ [Nt A] @ \<beta>) \<in> P)"
+(* reachable P S is the set of nonterminals reachable from the set of production
+rules P and set of start states S *)
 
-definition "rm_unreachable P = {(A,\<alpha>) | A \<alpha>. (A,\<alpha>) \<in> P \<and> reachable P A}"
+(*not sure if the inductive definition or the closure definition is better,
+I think both are correct, less confident about the closure definition being correct*)
+inductive_set reachable :: "('n,'t)Prods \<Rightarrow> 'n set \<Rightarrow> 'n set" for P S where
+"A \<in> S \<Longrightarrow> A \<in> reachable P S"
+| "\<lbrakk> (A,\<alpha>) \<in> P; A \<in> reachable P S; B \<in> nts_of_syms \<alpha>\<rbrakk> \<Longrightarrow> B \<in> reachable P S"
 
-lemma prefix_rm_unreachable: "rm_unreachable P \<subseteq> P"
+definition reachable_one_step :: "('n,'t)Prods \<Rightarrow> 'n set \<Rightarrow> 'n set" where
+"reachable_one_step P S = {A | A. \<exists>B \<alpha>. B \<in> S \<and> (B,\<alpha>) \<in> P \<and> A \<in> nts_of_syms \<alpha>}"
+
+definition "reachable_closure P S = closure (reachable_one_step P) S"
+
+definition "rm_unreachable P S = {(A,\<alpha>) | A \<alpha>. (A,\<alpha>) \<in> P \<and> A \<in> reachable_closure P S}"
+
+lemma mono_reachable_one_step: "mono reachable_one_step"
+unfolding reachable_one_step_def mono_def by (smt (verit, ccfv_SIG) Collect_mono le_funI subset_eq)
+
+
+
+
+
+lemma prefix_rm_unreachable: "rm_unreachable P S \<subseteq> P"
   unfolding rm_unreachable_def by auto
 
   text \<open>The main theorem:\<close>
 theorem 
-  assumes "reachable P A" 
-  shows "Lang (rm_unreachable P) A = Lang P A"
+  shows "Lang (rm_unreachable P {A}) A = Lang P A"
   proof
-    show "Lang (rm_unreachable P) A \<subseteq> Lang P A"
+    show "Lang (rm_unreachable P {A}) A \<subseteq> Lang P A"
       using Lang_mono prefix_rm_unreachable by metis
   next
-    show "Lang P A \<subseteq> Lang (rm_unreachable P) A"
-      using assms unfolding reachable_def rm_unreachable_def
+    show "Lang P A \<subseteq> Lang (rm_unreachable P {A}) A"
       sorry
 qed
 end
